lalloc for records. Mkpoint is extracted as an MLE_Ctor and not MLE_Record.

src/extraction/extractexp.fs
@@ -182,6 +182,22 @@ let normalize_abs e0 =
               else mk_Exp_abs(bs, e) None e0.pos in
    aux [] e0
 
+let ffi_mltuple_mlp (n:int) : mlpath = 
+    let name = if (1<n && n<6) then ("mktuple"^(Util.string_of_int n)) else (failwith "NYI in runtime/allocator/camlstack.mli") in
+    ["CamlStack"],name
+
+let fix_lalloc (arg (*the argument of lalloc (type arg is erased) *):mlexpr) : mlexpr = 
+match arg with
+| MLE_Tuple  args -> failwith "unexpected. Prims.TupleN is not specially handled yet. So, F* tuples, which are sugar forPrims.TupleN,  were expected to be extracted as MLE_CTor"
+| MLE_Record (mlns, fields) -> 
+    let args = List.map snd fields in 
+        let tup= (MLE_App (MLE_Name (ffi_mltuple_mlp (List.length args)), args)) in
+        let dummyTy = ml_unit_ty in
+        MLE_Coerce (tup,dummyTy,dummyTy) // if the pretty printing phase prints dummyTy, we will be in trouble
+| MLE_CTor (mlp, args) -> failwith "NYI: lalloc ctor" 
+| _ -> failwith "for efficiency, the argument to lalloc should be a head normal form of the type. Extraction will then avoid creating this value on the heap."
+
+
     
 (*Preconditions : 
    1) residualType is the type of mlAppExpr 
@@ -218,7 +234,7 @@ let maybe_lalloc_eta_data (g:env) (qual : option<fv_qual>) (residualType : mlty)
                     | _ -> failwith "Impossible" in
     
     match (mlAppExpr, qual) with
-        | (MLE_App (MLE_Name mlp, mlargs), _) when (mlp=mlp_lalloc) -> (debug g (fun () -> Util.print_string "need to do lalloc surgery here\n"));mlAppExpr
+        | (MLE_App (MLE_Name mlp, [mlarg]), _) when (mlp=mlp_lalloc) -> (debug g (fun () -> Util.print_string "need to do lalloc surgery here\n")); (fix_lalloc mlarg)
         | _, None -> mlAppExpr
         | MLE_App(MLE_Name mlp, mle::args), Some (Record_projector f) -> 
           let fn = Util.mlpath_of_lid f in
